Building the proof structure.

sepcomp/InliningproofEFF.v
@@ -25,16 +25,152 @@ Require Import effect_simulations_lemmas.
 Require Export Axioms.
 Require Import CminorSel_coop.
 Require Import RTL_eff.
+Require Import RTL_coop.
 
 Load Santiago_tactics.
 
-(*Definition MATCH (d:CMinSel_core) mu c1 m1 c2 m2:Prop :=
+Variable SrcProg: RTL.program.
+Variable TrgProg: RTL.program.
+Let SrcGe : RTL.genv := Genv.globalenv SrcProg.
+Let TrgGe : RTL.genv := Genv.globalenv TrgProg.
+
+(*LENB: GFP as in selectionproofEFF*)
+Definition globalfunction_ptr_inject (j:meminj):=
+  forall b f, Genv.find_funct_ptr SrcGe b = Some f -> 
+              j b = Some(b,0) /\ isGlobalBlock SrcGe b = true. 
+
+(*The new match_states*)
+Inductive match_states (j:meminj): RTL_core -> mem -> RTL_core -> mem -> Prop :=
+  | match_state:
+      forall f s k sp e m tm cs tf ns rs (*map ncont nexits ngoto nret rret*) sp'
+        (*(MWF: map_wf map)*)
+        (*(TS: tr_stmt tf.(fn_code) map s ns ncont nexits ngoto nret rret)*)
+        (*(TF: tr_fun tf map f ngoto nret rret)*)
+        (*(TK: tr_cont j tf.(fn_code) map k ncont nexits ngoto nret rret cs)*)
+        (*(ME: match_env j map e nil rs)*)
+        (*(MEXT: Mem.extends m tm)*)
+        (MINJ: Mem.inject j m tm)
+        (*(*NEW:*) (SP: sp_preserved j sp sp')*),
+      match_states j (RTL_State f s k sp e) m
+                     (RTL_State cs tf sp' ns rs) tm
+  | match_callstate:
+      forall f args targs k m tm cs tf
+        (*(TF: transl_fundef f = OK tf)*)
+        (*(MS: match_stacks j k cs)*)
+        (*(LD: Val.lessdef_list args targs)*)
+        (*(AINJ: val_list_inject j args targs)*)
+        (*(MEXT: Mem.extends m tm)*)
+        (*(MINJ: Mem.inject j m tm)*),
+      match_states j (RTL_Callstate f args k) m
+                     (RTL_Callstate cs tf targs) tm
+  | match_returnstate:
+      forall v tv k m tm cs
+        (*(MS: match_stacks j k cs)*)
+        (*(LD: Val.lessdef v tv)*)
+         (*(VINJ: val_inject j v tv)*)
+        (*(MEXT: Mem.extends m tm)*)
+        (*(MINJ: Mem.inject j m tm)*),
+      match_states j (RTL_Returnstate v k) m
+                     (RTL_Returnstate cs tv) tm.
+
+Print restrict.
+Definition MATCH (d:RTL_core) mu c1 m1 c2 m2:Prop :=
+  match_states (restrict (as_inj mu) (vis mu)) c1 m1 c2 m2 /\
+  REACH_closed m1 (vis mu) /\
+  meminj_preserves_globals SrcGe (as_inj mu) /\
+  globalfunction_ptr_inject (as_inj mu) /\
+  (forall b, isGlobalBlock SrcGe b = true -> frgnBlocksSrc mu b = true) /\
+  sm_valid mu m1 m2 /\ SM_wd mu /\ Mem.inject (as_inj mu) m1 m2.
+
+
+(** The simulation proof *)
+Theorem transl_program_correct:
+  forall (R: list_norepet (map fst (prog_defs SrcProg)))
+         entrypoints
+         (entry_points_ok : 
+            forall v1 v2 sig,
+              In (v1, v2, sig) entrypoints -> 
+              exists b f1 f2, 
+                v1 = Vptr b Int.zero 
+                /\ v2 = Vptr b Int.zero
+                /\ Genv.find_funct_ptr SrcGe b = Some f1
+                /\ Genv.find_funct_ptr TrgGe b = Some f2)
+         (init_mem: exists m0, Genv.init_mem SrcProg = Some m0),
+SM_simulation.SM_simulation_inject rtl_eff_sem
+   rtl_eff_sem SrcGe TrgGe entrypoints.
+
+intros.
+eapply sepcomp.effect_simulations_lemmas.inj_simulation_star_wf.
+Lemma genvs_domain_eq_implication: (exists m0:mem, Genv.init_mem SrcProg = Some m0) -> 
+genvs_domain_eq SrcGe TrgGe.
+Admitted.
+apply genvs_domain_eq_implication; auto.
+Lemma match_correspondance: forall (d : RTL_core) (mu : SM_Injection) (c1 : RTL_core) 
+     (m1 : mem) (c2 : RTL_core) (m2 : mem), MATCH d mu c1 m1 c2 m2 -> SM_wd mu.
+Admitted.
+eapply match_correspondance.
+Lemma match_to_reach: forall (d : RTL_core) (mu : SM_Injection) (c1 : RTL_core) 
+     (m1 : mem) (c2 : RTL_core) (m2 : mem),
+   MATCH d mu c1 m1 c2 m2 -> REACH_closed m1 (vis mu).
+Admitted.
+apply match_to_reach.
+
+
+
+
+
+Record map_wf (m: mapping) : Prop :=
+  mk_map_wf {
+    map_wf_inj:
+      (forall id1 id2 r,
+         m.(map_vars)!id1 = Some r -> m.(map_vars)!id2 = Some r -> id1 = id2);
+     map_wf_disj:
+      (forall id r,
+         m.(map_vars)!id = Some r -> In r m.(map_letvars) -> False)
+  }.
+
+Inductive match_states (j:meminj): CMinSel_core -> mem -> RTL_core -> mem -> Prop :=
+  | match_state:
+      forall f s k sp e m tm cs tf ns rs map ncont nexits ngoto nret rret sp'
+        (MWF: map_wf map)
+        (TS: tr_stmt tf.(fn_code) map s ns ncont nexits ngoto nret rret)
+        (TF: tr_fun tf map f ngoto nret rret)
+        (TK: tr_cont j tf.(fn_code) map k ncont nexits ngoto nret rret cs)
+        (ME: match_env j map e nil rs)
+        (*(MEXT: Mem.extends m tm)*)
+        (MINJ: Mem.inject j m tm)
+        (*NEW:*) (SP: sp_preserved j sp sp'),
+      match_states j (CMinSel_State f s k sp e) m
+                     (RTL_State cs tf sp' ns rs) tm
+  | match_callstate:
+      forall f args targs k m tm cs tf
+        (TF: transl_fundef f = OK tf)
+        (MS: match_stacks j k cs)
+        (*(LD: Val.lessdef_list args targs)*)
+        (AINJ: val_list_inject j args targs)
+        (*(MEXT: Mem.extends m tm)*)
+        (MINJ: Mem.inject j m tm),
+      match_states j (CMinSel_Callstate f args k) m
+                     (RTL_Callstate cs tf targs) tm
+  | match_returnstate:
+      forall v tv k m tm cs
+        (MS: match_stacks j k cs)
+        (*(LD: Val.lessdef v tv)*)
+         (VINJ: val_inject j v tv)
+        (*(MEXT: Mem.extends m tm)*)
+        (MINJ: Mem.inject j m tm),
+      match_states j (CMinSel_Returnstate v k) m
+                     (RTL_Returnstate cs tv) tm.
+
+
+
+Definition MATCH (d:RTL_core) mu c1 m1 c2 m2:Prop :=
   match_states (restrict (as_inj mu) (vis mu)) c1 m1 c2 m2 /\
   REACH_closed m1 (vis mu) /\
   meminj_preserves_globals ge (as_inj mu) /\
   globalfunction_ptr_inject (as_inj mu) /\
   (forall b, isGlobalBlock ge b = true -> frgnBlocksSrc mu b = true) /\
-  sm_valid mu m1 m2 /\ SM_wd mu /\ Mem.inject (as_inj mu) m1 m2.*)
+  sm_valid mu m1 m2 /\ SM_wd mu /\ Mem.inject (as_inj mu) m1 m2.
 
 Print effstep.
 Print rtl_eff_sem.
